src/lowparse/LowParse.Spec.Sum.fst
@@ -251,15 +251,13 @@ let make_sum_with_nondep
   (s: sum)
 = Sum (sum_key_type s) (sum_repr_type s) (sum_enum s) (nondep_part * sum_type s) (tag_of_data_with_nondep nondep_part (sum_tag_of_data s))
 
-#set-options "--use_two_phase_tc false"
-
 inline_for_extraction
 val synth_sum_with_nondep_case
   (nondep_part: Type0)
   (t: sum)
   (x: sum_key (make_sum_with_nondep nondep_part t))
-  (d: nondep_part * sum_cases t (let x : sum_key_type t = x in x))
-: Tot (sum_cases (make_sum_with_nondep nondep_part t) (let x : sum_key_type t = x in x))
+  (d: nondep_part * sum_cases t (coerce' (sum_key t) x))
+: Tot (sum_cases (make_sum_with_nondep nondep_part t) x)
 
 let synth_sum_with_nondep_case nondep_part t x d
 = match d with
@@ -267,8 +265,6 @@ let synth_sum_with_nondep_case nondep_part t x d
     [@inline_let]
     let ds : sum_type t = ds in
     (df, ds)
-
-#reset-options
 
 let parse_sum_with_nondep_cases
   (#nondep_part: Type0)
